Add cleaner version of state_interp

src/Examples/Logging/LogRefinement.v
@@ -35,9 +35,9 @@ Section refinement_triples.
      | Txn12 => (∃ txn1 txn2, ⌜txns = [txn1; txn2]⌝ ∗
                                                  txn_map txn1_start txn1 ∗
                                                  txn_map txn2_start txn2)
-     | Txn21 => ∃ txn1 txn2, ⌜txns = [txn1; txn2]⌝ ∗
-                                                txn_map txn2_start txn1 ∗
-                                                txn_map txn1_start txn2
+     | Txn21 => ∃ txn1 txn2, ⌜txns = [txn2; txn1]⌝ ∗
+                                                txn_map txn1_start txn1 ∗
+                                                txn_map txn2_start txn2
      end)%I.
 
   Definition txn_free start :=
@@ -54,6 +54,34 @@ Section refinement_triples.
 
   Definition state_interp (s:BufState) (txns: list (nat*nat)) :=
     (buffer_map s txns ∗ free_buffer_map s)%I.
+
+  Definition state_interp' (s:BufState) (txns: list (nat*nat)) :=
+    (match s with
+     | Empty => ⌜txns = []⌝ ∗ txn_free txn1_start ∗ txn_free txn2_start
+     | Txn1 => ∃ txn1, ⌜txns = [txn1]⌝ ∗ txn_map txn1_start txn1 ∗ txn_free txn2_start
+    | Txn2 => ∃ txn2, ⌜txns = [txn2]⌝ ∗ txn_map txn2_start txn2 ∗ txn_free txn1_start
+    | Txn12 => ∃ txn1 txn2, ⌜txns = [txn1; txn2]⌝ ∗ txn_map txn1_start txn1 ∗ txn_map txn2_start txn2
+    | Txn21 => ∃ txn1 txn2, ⌜txns = [txn2; txn1]⌝ ∗ txn_map txn1_start txn1 ∗ txn_map txn2_start txn2
+     end)%I.
+
+  Theorem state_interp_to_state_interp' s txns :
+    state_interp s txns -∗ state_interp' s txns.
+  Proof.
+    unfold state_interp; destruct s; simpl; iIntros "H".
+    - auto.
+    - iDestruct "H" as "(H1&H2)".
+      iDestruct "H1" as (txn ->) "H1".
+      iExists _; by iFrame.
+    - iDestruct "H" as "(H1&H2)".
+      iDestruct "H1" as (txn ->) "H1".
+      iExists _; by iFrame.
+    - iDestruct "H" as "(H1&H2)".
+      iDestruct "H1" as (txn1 txn2 ->) "H1".
+      iExists _, _; by iFrame.
+    - iDestruct "H" as "(H1&H2)".
+      iDestruct "H1" as (txn1 txn2 ->) "H1".
+      iExists _, _; by iFrame.
+  Qed.
 
   Record ghost_names :=
     { γslock : gname;
@@ -385,8 +413,8 @@ Section refinement_triples.
       iApply "HΦ".
       iExists s', txns.
       (* use reserve_state_ok to get the garbage transaction we're reserving *)
-      iPoseProof (reserve_state_ok with "Hstateinterp") as "Hstateinterp"; eauto.
-      iDestruct "Hstateinterp" as (txn0) "(Htxn0&Hwand)".
+      iPoseProof (reserve_state_ok with "Hstateinterp") as "Hreserved"; eauto.
+      iDestruct "Hreserved" as (txn0) "(Htxn0&Hwand)".
       iExists txn0.
       iFrame.
       auto.
@@ -488,11 +516,11 @@ Section refinement_triples.
        wp_lock "(Hslocked & Hstateinv)".
        wp_bind.
        iDestruct "Hstateinv" as (s txns') "(Hstate&Hstateinterp&Howntxn)".
+       iPoseProof (state_interp_to_state_interp' with "Hstateinterp") as "Hstateinterp".
        iApply (get_state_ok with "Hstate"). iIntros "!> Hstate".
        wp_bind.
-       destruct s.
-       * simpl.
-         replace (length log + 0) with (length log) by lia.
+       destruct s; simpl.
+       * replace (length log + 0) with (length log) by lia.
          wp_step.
          wp_bind.
          iInv "Hinv" as (txns'' log') ">(Hvol&Hdur&Habs)".
